theory Attempts
  imports FormalLanguages
  imports CommunicatingAutomata
begin

subsubsection "influenced language approaches 1"

inductive path_to_root :: "'peer â‡’ 'peer list â‡’ bool" where
PTRRoot: "ð’«â‡©?(p) = {} âŸ¹ path_to_root p [p]" |
PTRNode: "âŸ¦ð’«â‡©?(p) = {q}; path_to_root q asâŸ§ âŸ¹ path_to_root p (p # as)"

fun is_root :: "'peer topology â‡’ 'peer â‡’ bool" where
"is_root E p = ((card (EâŸ¨â†’pâŸ©)) = 0) "

fun get_root :: "'peer topology â‡’ 'peer" where
"get_root E = (THE x. is_root E x)"

fun get_path_to_root :: "'peer â‡’  'peer list" where
"get_path_to_root p = (THE ps. path_to_root p ps)"

fun infl_lang_rec :: "'peer list â‡’ ('information, 'peer) action language" where
"infl_lang_rec [] = {}" |
"infl_lang_rec [r] = {Îµ}" |
"infl_lang_rec (p # q # ps) = {w | w. w âˆˆ â„’(p) âˆ§ (wâ†“â‡©?)â†“â‡©!â‡©? âˆˆ ((infl_lang_rec (q # ps))â‡‚â‡©! )â‡‚â‡©!â‡©? âˆ§ ð’«â‡©?(p) = {q}}" 

fun infl_lang :: "'peer list â‡’ ('information, 'peer) action language" where
"infl_lang [] = {}" |
"infl_lang [r] = â„’(r)" |
"infl_lang ps = infl_lang_rec ps" 

abbreviation InfluencedLanguage :: "'peer â‡’ ('information, 'peer) action language"  ("â„’â‡§* _" [90] 100) where
"â„’â‡§* p â‰¡ infl_lang (get_path_to_root p)"

abbreviation InfluencedLanguageSend :: "'peer â‡’ ('information, 'peer) action language"  ("â„’â‡©!â‡§* _" [90] 100) where
"â„’â‡©!â‡§* p â‰¡ (â„’â‡§* p)â‡‚â‡©! "

abbreviation InfluencedLanguageRecv :: "'peer â‡’ ('information, 'peer) action language"  ("â„’â‡©?â‡§* _" [90] 100) where
"â„’â‡©?â‡§* p â‰¡ (â„’â‡§* p)â‡‚â‡©! "


subsubsection "influenced language approaches 2"
text "test and test2 should do the same but I am not 100% sure (hence why I try to prove it with eqtest "

inductive test :: "'peer â‡’ ('information, 'peer) action word â‡’ bool" where
t0 : "âŸ¦ð’«â‡©?(r) = {}; w âˆˆ â„’(r)âŸ§ âŸ¹ test r w" |
t1 : "âŸ¦ð’«â‡©?(r) = {}; ð’«â‡©?(q) = {r}; w âˆˆ â„’(q); ((wâ†“â‡©?)â†“â‡©!â‡©?) âˆˆ ((â„’(r))â‡‚â‡©!â‡©?) âŸ§ âŸ¹ test q w" |
t2 : "âŸ¦ð’«â‡©?(p) = {q}; w âˆˆ â„’(p); w' âˆˆ â„’(q); test q w'; ((wâ†“â‡©?)â†“â‡©!â‡©?) = ((w'â†“â‡©!)â†“â‡©!â‡©?); ((wâ†“â‡©?)â†“â‡©!â‡©?) âˆˆ (((â„’(q))â‡‚â‡©!)â‡‚â‡©!â‡©?)âŸ§ âŸ¹ test p w"

inductive test2 :: "'peer â‡’ ('information, 'peer) action word â‡’ bool" where
t00: "âŸ¦ð’«â‡©?(r) = {}; w âˆˆ â„’(r)âŸ§ âŸ¹ test2 r w" | â€•â€¹influenced language of root r is language of râ€º
t10: "âŸ¦ð’«â‡©?(r) = {}; ð’«â‡©?(q) = {r}; w âˆˆ â„’(q); ((wâ†“â‡©?)â†“â‡©!â‡©?) âˆˆ ((â„’(r))â‡‚â‡©!â‡©?) âŸ§ âŸ¹ test2 q w" | â€•â€¹q is direct child of root râ€º
t20: "âŸ¦ð’«â‡©?(p) = {q}; w âˆˆ â„’(p); test2 q w'; ((wâ†“â‡©?)â†“â‡©!â‡©?) = ((w'â†“â‡©!)â†“â‡©!â‡©?)âŸ§ âŸ¹ test2 p w" â€•â€¹p is any node and q its parentâ€º

lemma eeeeee : "test2 p w âŸ¹  w âˆˆ â„’(p)" using test2.induct by simp
lemma eeeeeee : "âŸ¦ð’«â‡©?(p) = {q}; w âˆˆ â„’(p); test2 q w'; ((wâ†“â‡©?)â†“â‡©!â‡©?) = ((w'â†“â‡©!)â†“â‡©!â‡©?)âŸ§ âŸ¹ ((wâ†“â‡©?)â†“â‡©!â‡©?) âˆˆ (((â„’(q))â‡‚â‡©!)â‡‚â‡©!â‡©?)" 
  using eeeeee by blast
text "this means test and test2 are equivalent, test2 is just shorter"

lemma "âŸ¦x = 2; y = x + 1; y > x; y < 5âŸ§ âŸ¹ y = 3" by auto

lemma eqtest : "test2 p w âŸ¹ test p w"
proof (induction rule:test2.induct)
  case (t00 r w)
  then show ?case 
    by (simp add: t0)
next
  case (t10 r q w)
  then show ?case 
    by (simp add: t1)
next
  case (t20 p q w w')
  then show ?case sorry
qed

abbreviation infl_lang2 :: "'peer â‡’ ('information, 'peer) action language" where
"infl_lang2 p â‰¡ {w | w. test p w}"

value "[!âŸ¨xâŸ©, ?âŸ¨yâŸ©, ?âŸ¨zâŸ©]"
value "let w = [!âŸ¨xâŸ©, ?âŸ¨yâŸ©, ?âŸ¨zâŸ©] in ((wâ†“â‡©?)â†“â‡©!â‡©?)"
value "let w' = [?âŸ¨aâŸ©, !âŸ¨yâŸ©, !âŸ¨zâŸ©] in ((w'â†“â‡©!)â†“â‡©!â‡©?)"


lemma filter_head : 
  assumes "xs â‰  []" and "x = hd xs" and "x = hd (filter f (xs))"
  shows "f x"
proof (rule ccontr)
  assume "Â¬ (f x)"
  then show "False"
  proof
    have "filter f [x] = []" by (simp add: â€¹Â¬ f xâ€º)
    moreover obtain ys where "xs = (x # ys)" by (metis assms(1,2) list.collapse)
    moreover have "filter f xs = filter f ys" by (simp add: â€¹Â¬ f xâ€º calculation(2))
    moreover have "x = hd (filter f ys)" by (simp add: assms(3) calculation(3))
    moreover have "filter f xs = filter f (filter f xs)" by simp
    moreover have "filter f (x # ys) = filter f (filter f (x # ys))" by simp
    moreover have "filter f xs = filter f ys" using calculation(3) by blast
    moreover have "hd (filter f ys) = hd (filter f xs)"  by (simp add: calculation(3))
    moreover have "hd (filter f ys) = hd (filter f (x # ys))" using assms(3) calculation(2,4) by argo
    moreover have "xs â‰  ys" by (simp add: calculation(2))
    ultimately show "f x" sorry
qed
qed


end